concurrency/hack-hash-table/MapSpec.s.dfy
@@ -1,0 +1,113 @@
+module KeyValueType {
+  type Key = uint64
+  type Value(==)
+}
+
+module InputOutputIfc {
+  type Input(!new)
+  type Output(!new)
+
+  datatype Op = Op(input: Input, output: Output)
+}
+
+module MapIfc refines InputOutputIfc {
+  import opened KeyValueType
+
+  datatype Input =
+    | QueryInput(key: Key)
+    | InsertInput(key: Key, value: Value)
+
+  datatype Output =
+    | QueryOutput(value: Value)
+    | InsertOutput
+}
+
+module AsyncIfc {
+  import Ifc = MapIfc
+  type {:extern} RequestId(==,!new)
+
+  datatype Op =
+    | Start(rid: RequestId, input: Ifc.Input)
+    | End(rid: RequestId, output: Ifc.Output)
+    | InternalOp
+}
+
+// disallowed:
+
+// thread 1 : 4 butter, 2 sugar
+// thread 2 : 2 butter, 4 sugar
+
+// thread 1 : 3 batches returned
+// thread 2 : 3 batches returned
+
+module MapSpec {
+  import Ifc = MapIfc
+  datatype Variables = Variables(butter: nat, sugar: nat)
+
+  predicate Init(s: Variables) {
+    && s.butter == 0
+    && s.sugar == 0
+  }
+
+  predicate Next(s: Variables, s': Variables, op: Ifc.Op) {
+    match op {
+      case Op(input, output) => (
+        exists num_batches: nat ::
+          && num_batches <= s.butter + input.butter
+          && num_batches <= s.sugar + input.sugar
+          && s'.butter == s.butter + input.butter - num_batches
+          && s'.sugar == s.sugar + input.sugar - num_batches
+          && output == Ifc.Output(6 * num_batches)
+      )
+    }
+  }
+}
+
+module AsyncSpec {
+  import InnerIfc = CookieIfc
+  import SM = CookieSpec
+  import Ifc = AsyncIfc
+
+  type RequestId = Ifc.RequestId
+
+  datatype Req = Req(rid: RequestId, input: InnerIfc.Input)
+  datatype Resp = Req(rid: RequestId, input: InnerIfc.Input)
+
+  datatype Variables = Variables(
+      s: SM.Variables,
+      reqs: multiset<Req>,
+      resps: multiset<Resp>)
+
+  predicate Init(s: Variables)
+  {
+    && SM.Init(s.s)
+    && s.reqs == multiset{}
+    && s.resps == multiset{}
+  }
+
+  predicate Next(s: Variables, s': Variables, op: Ifc.Op)
+  {
+    match op {
+      case Start(rid, input) =>
+        // add 'input' to 'reqs'
+        && s' == s.(reqs := s.reqs + multiset{Req(rid, input)})
+      case InternalOp => (
+        // stutter step
+        || (s' == s)
+        // resolve request step
+        // serialization point: remove 'input' from 'reqs',
+        // add 'output' to 'resps'
+        || (exists rid, input, output ::
+          && Req(rid, input) in s.reqs
+          && s'.reqs == s.reqs - multiset{Req(rid, input)}
+          && s'.resps == s.resps + multiset{Resp(rid, output)}
+          && SM.Next(s.s, s'.s, InnerIfc.Op(input, output))
+        )
+      )
+      case End(rid, output) =>
+        // remove from 'resps'
+        && Resp(rid, output) in s.resps
+        && s' == s.(resps := s'.resps - multiset{Resp(rid, output)})
+    }
+  }
+}
